Hitting a performance problem

example/Deed.thy
@@ -13,14 +13,13 @@ solidity: 2d9109ba453d49547778c39a506b0ed492305c16
 $ solc/solc --bin-runtime
 *)
 
-(*
 abbreviation deed :: "char list"
 where "deed == ''6060604052361561006c5760e060020a600035046305b34410811461006e5780630b5ab3d51461007c57806313af4035146100895780632b20e397146100af5780638da5cb5b146100c6578063bbe42771146100dd578063faab9d3914610103578063fb1669ca14610129575b005b346100025761014a60015481565b346100025761006c610189565b346100025761006c60043560005433600160a060020a039081169116146101f857610002565b34610002576101a0600054600160a060020a031681565b34610002576101a0600254600160a060020a031681565b346100025761006c60043560005433600160a060020a0390811691161461025757610002565b346100025761006c60043560005433600160a060020a039081169116146102c757610002565b61006c60043560005433600160a060020a039081169116146102e957610002565b60408051918252519081900360200190f35b6040517fbb2ce2f51803bba16bc85282b47deeea9a5c6223eabea1077be696b3f265cf1390600090a16102545b60025460a060020a900460ff16156101bd57610002565b60408051600160a060020a03929092168252519081900360200190f35b604051600254600160a060020a0390811691309091163180156108fc02916000818181858888f19350505050156101f35761deadff5b610002565b6002805473ffffffffffffffffffffffffffffffffffffffff19168217905560408051600160a060020a038316815290517fa2ea9883a321a3e97b8266c2b078bfeec6d50c711ed71f874a90d500ae2eaf369181900360200190a15b50565b60025460a060020a900460ff16151561026f57610002565b6002805474ff00000000000000000000000000000000000000001916905560405161dead906103e830600160a060020a031631848203020480156108fc02916000818181858888f19350505050151561015c57610002565b6000805473ffffffffffffffffffffffffffffffffffffffff19168217905550565b60025460a060020a900460ff16151561030157610002565b8030600160a060020a031631101561031857610002565b600254604051600160a060020a039182169130163183900380156108fc02916000818181858888f1935050505015156102545761000256''"
-*)
 
+(*
 abbreviation deed :: "char list"
 where "deed == ''6060604052361561006c5760e060020a600035046305b344108114''"
-
+*)
 
 abbreviation "deed_bytes == bytes_of_hex_content deed"
 
@@ -29,11 +28,22 @@ where "deed_insts == fst (the (parse_bytes deed_bytes))"
 
 value "parse_bytes deed_bytes"
 
+abbreviation deed_program :: "program"
+where
+"deed_program == program_of_lst deed_insts"
+
+value deed_program
+
 inductive deed_inv :: "account_state \<Rightarrow> bool"
 where
-" account_code a = program_of_lst deed_insts \<Longrightarrow>
+" account_code a = deed_program \<Longrightarrow>
   deed_inv a
 "
+
+lemma dlen : "program_length deed_program = 500"
+apply(simp)
+
+oops
 
 lemma deed_keeps_invariant :
 "no_assertion_failure deed_inv"
@@ -44,32 +54,9 @@ apply(rule impI)
 apply(rule allI)
 apply(rule impI)
 apply(drule star_case)
-apply(simp add: deed_inv.simps)
-apply(simp add: one_step.simps add: world_turn.simps; auto)
- apply(simp add: contract_turn.simps; auto)
-  apply(drule star_case)
-  apply(case_tac steps; auto)
-   apply(simp split: if_splits)
-  apply(simp split: if_splits)
-  apply(drule star_case; auto)
-   apply(drule one_step.cases; auto)
-   apply(drule world_turn.cases; auto)
-  apply(drule one_step.cases; auto)
-  apply(drule world_turn.cases; auto)
- apply(drule star_case; auto)
- apply(drule one_step.cases; auto)
- apply(drule world_turn.cases; auto)
-apply(drule star_case; auto)
- apply(drule contract_turn.cases; auto)
- apply(case_tac steps; auto)
- apply(simp split: if_splits)
-apply(drule contract_turn.cases; auto)
- apply(case_tac steps; auto)
- apply(simp split: if_splits)
- apply(drule one_step.cases; auto)
- apply(drule world_turn.cases; auto)
-apply(drule one_step.cases; auto)
-apply(drule world_turn.cases; auto)
-done
-     
+apply(drule deed_inv.cases)
+apply(simp)
+
+oops
+
 end
